Foundation/Modal/Kripke2/Grz/Soundness.lean
@@ -1,0 +1,24 @@
+import Foundation.Modal.ComplementClosedConsistentFinset
+import Foundation.Modal.Hilbert2.WellKnown
+import Foundation.Modal.Kripke2.AxiomGrz
+import Foundation.Modal.Kripke2.KT
+import Foundation.Modal.Kripke2.Soundness
+import Foundation.Modal.System.Grz
+
+namespace LO.Modal
+
+namespace Hilbert.Grz
+
+open Formula
+open Formula.Kripke
+open System
+open System.Context
+open ComplementClosedConsistentFinset
+
+instance Kripke.consistent : System.Consistent (Hilbert.Grz) := by
+  -- haveI := FrameClass.definedBy_with_axiomK TransitiveIrreflexiveFiniteFrameClass.DefinedByL
+  sorry;
+
+end Hilbert.Grz
+
+end LO.Modal
